Examples.lean
@@ -2,6 +2,7 @@ import Examples.Pow.Correct
 import Examples.Truth.Correct
 import Examples.Caller.Correct
 import Examples.ERC20.Correct
+import Examples.StorageBackendTests
 import Examples.CtorTruth.Correct
 import Examples.CtorStore.Correct
 import Examples.TinyImmutable.Correct
