Solm.lean
@@ -3,4 +3,6 @@ import Solm.Notation
 import Solm.Value
 import Solm.Storage
 import Solm.Semantics
+import Solm.MetaSolidityLayout
+import Solm.StorageLaws
 import Solm.Immutables
